Started even more tedious refactoring.
Changed the structure of the cenv (and it's tenvC counterpart). It used
to be something like ((modN option * conN) * 'a) list and now it's
structure more closely resembles the module structure of the program
(modN * (conN * 'a) list) list * (conN * 'a) list

The idea is the the operations that put constructors into modules will
be much easier to reason about then before, where ad hoc code traversed
the cenv and changed the domain.

metatheory/typeSysPropsScript.sml
@@ -9,6 +9,8 @@ val check_dup_ctors_def = semanticPrimitivesTheory.check_dup_ctors_def;
 val build_tdefs_def = semanticPrimitivesTheory.build_tdefs_def;
 val find_recfun_def = semanticPrimitivesTheory.find_recfun_def;
 val same_tid_def = semanticPrimitivesTheory.same_tid_def;
+val lookup_con_id_def = semanticPrimitivesTheory.lookup_con_id_def;
+val merge_envC_def = semanticPrimitivesTheory.merge_envC_def;
 
 val all_distinct_map_inj = Q.prove (
 `!f l. (!x y. (f x = f y) ⇒ (x = y)) ⇒ (ALL_DISTINCT (MAP f l) = ALL_DISTINCT l)`,
@@ -38,14 +40,27 @@ val disjoint_env_def = Define `
   disjoint_env e1 e2 =
     DISJOINT (set (MAP FST e1)) (set (MAP FST e2))`;
 
-val tenvC_ok_merge = Q.store_thm ("tenvC_ok_merge",
+val flat_tenvC_ok_merge = Q.prove (
 `!tenvC1 tenvC2.
-  tenvC_ok (merge tenvC1 tenvC2) = 
-  (tenvC_ok tenvC1 ∧ tenvC_ok tenvC2)`, 
-rw [tenvC_ok_def, merge_def, ALL_DISTINCT_APPEND] >>
+  flat_tenvC_ok (merge tenvC1 tenvC2) = 
+  (flat_tenvC_ok tenvC1 ∧ flat_tenvC_ok tenvC2)`, 
+rw [flat_tenvC_ok_def, merge_def, ALL_DISTINCT_APPEND] >>
 eq_tac >>
 rw [disjoint_env_def, DISJOINT_DEF, EXTENSION] >>
 metis_tac []);
+
+val tenvC_ok_merge = Q.store_thm ("tenvC_ok_merge",
+`!tenvC1 tenvC2.
+  tenvC_ok (merge_tenvC tenvC1 tenvC2) = 
+  (tenvC_ok tenvC1 ∧ tenvC_ok tenvC2)`, 
+ rw [] >>
+ PairCases_on `tenvC1` >>
+ PairCases_on `tenvC2` >>
+ rw [tenvC_ok_def, merge_tenvC_def, ALL_DISTINCT_APPEND] >>
+ eq_tac >>
+ rw [merge_def, EVERY_MEM] >>
+ res_tac >>
+ metis_tac [flat_tenvC_ok_merge, merge_def]);
 
 val tenvCT_ok_merge = Q.store_thm ("tenvCT_ok_merge",
 `!tenvC1 tenvC2.
@@ -56,19 +71,65 @@ eq_tac >>
 rw [disjoint_env_def, DISJOINT_DEF, EXTENSION] >>
 metis_tac []);
 
-val tenvC_ok_lookup = Q.store_thm ("tenvC_ok_lookup",
+val flat_tenvC_ok_lookup = Q.prove (
 `!tenvC cn tvs ts tn.
-  tenvC_ok tenvC ∧ (lookup cn tenvC = SOME (tvs,ts,tn))
+  flat_tenvC_ok tenvC ∧ (lookup cn tenvC = SOME (tvs,ts,tn))
   ⇒
   EVERY (check_freevars 0 tvs) ts`,
 induct_on `tenvC` >>
 rw [] >>
 PairCases_on `h` >>
-fs [tenvC_ok_def] >>
+fs [flat_tenvC_ok_def] >>
 every_case_tac >>
 rw [] >>
 fs [] >>
 metis_tac []);
+
+val lookup_in = Q.store_thm ("lookup_in",
+`!x e v. (lookup x e = SOME v) ⇒ MEM v (MAP SND e)`,
+induct_on `e` >>
+rw [lookup_def] >>
+cases_on `h` >>
+fs [lookup_def] >>
+every_case_tac >>
+fs [] >>
+metis_tac []);
+
+val lookup_in2 = Q.store_thm ("lookup_in2",
+`!x e v. (lookup x e = SOME v) ⇒ MEM x (MAP FST e)`,
+induct_on `e` >>
+rw [lookup_def] >>
+cases_on `h` >>
+fs [lookup_def] >>
+every_case_tac >>
+fs [] >>
+metis_tac []);
+
+val tenvC_ok_lookup = Q.store_thm ("tenvC_ok_lookup",
+`!tenvC cn tvs ts tn.
+  tenvC_ok tenvC ∧ (lookup_con_id cn tenvC = SOME (tvs,ts,tn))
+  ⇒
+  EVERY (check_freevars 0 tvs) ts`,
+ cases_on `cn` >>
+ rw [] >>
+ PairCases_on `tenvC` >>
+ fs [lookup_con_id_def, tenvC_ok_def]
+ >- metis_tac [flat_tenvC_ok_lookup] >> 
+ every_case_tac >>
+ fs [] >>
+ imp_res_tac lookup_in >>
+ fs [MEM_MAP, EVERY_MEM] >>
+ rw [] >>
+ PairCases_on `y` >>
+ fs [] >>
+ rw [] >>
+ PairCases_on `y'` >>
+ fs [] >>
+ rw [] >>
+ res_tac >>
+ fs [] >>
+ imp_res_tac flat_tenvC_ok_lookup >>
+ fs [EVERY_MEM]);
 
 val tenvCT_ok_lookup = Q.store_thm ("tenvCT_ok_lookup",
 `!tenvCT cn tvs ts tn.
@@ -120,26 +181,6 @@ val type_ps_length = Q.store_thm ("type_ps_length",
 induct_on `ps` >>
 rw [Once type_p_cases] >>
 rw [] >>
-metis_tac []);
-
-val lookup_in = Q.store_thm ("lookup_in",
-`!x e v. (lookup x e = SOME v) ⇒ MEM v (MAP SND e)`,
-induct_on `e` >>
-rw [lookup_def] >>
-cases_on `h` >>
-fs [lookup_def] >>
-every_case_tac >>
-fs [] >>
-metis_tac []);
-
-val lookup_in2 = Q.store_thm ("lookup_in2",
-`!x e v. (lookup x e = SOME v) ⇒ MEM x (MAP FST e)`,
-induct_on `e` >>
-rw [lookup_def] >>
-cases_on `h` >>
-fs [lookup_def] >>
-every_case_tac >>
-fs [] >>
 metis_tac []);
 
 val lookup_disjoint = Q.store_thm ("lookup_disjoint",
@@ -1288,9 +1329,9 @@ rw [lookup_def,lookup_append_none]);
 
 val lookup_none_lem = Q.prove (
 `!x h0 h1 h2 h3.
-  (lookup x (MAP (λ(cn,ts). (Short cn,h0,ts,TypeId (mk_id mn h1))) h2) = NONE)
+  (lookup x (MAP (λ(cn,ts). (cn,h0,ts,TypeId (mk_id mn h1))) h2) = NONE)
   = 
-  (lookup x (MAP (λ(conN,ts). (Short conN,LENGTH ts,TypeId (mk_id mn h3))) h2) = NONE)`,
+  (lookup x (MAP (λ(conN,ts). (conN,LENGTH ts,TypeId (mk_id mn h3))) h2) = NONE)`,
 induct_on `h2` >>
 rw [lookup_def] >>
 PairCases_on `h` >>
@@ -1313,54 +1354,109 @@ val lookup_none = Q.store_thm ("lookup_none",
  >- metis_tac [lookup_none_lem]
  >- metis_tac [build_ctor_tenv_def, build_tdefs_def, lookup_reverse_none]);
 
+ (*
 val consistent_con_append = Q.store_thm ("consistent_con_append",
-`!tenvTC envC tenvC.
-  consistent_con_env tenvTC envC tenvC ⇒
-    ∀envC' tenvC'.
-      consistent_con_env tenvTC envC' tenvC'
-      ⇒
-      consistent_con_env tenvTC (envC++envC') (tenvC++tenvC')`,
-rw [consistent_con_env_def, lookup_append] >>
-every_case_tac >>
-rw [] >>
-res_tac >>
-fs [] >>
-metis_tac [tenvC_ok_merge, merge_def]);
+`!tenvTC envC tenvC envC' tenvC'.
+  consistent_con_env tenvTC envC tenvC ∧
+  consistent_con_env tenvTC envC' tenvC'
+  ⇒
+  consistent_con_env tenvTC (merge_envC envC envC') (merge_tenvC tenvC tenvC')`,
+
+
+ rw [consistent_con_env_def, lookup_append]
+ >- metis_tac [tenvC_ok_merge] >>
+ rpt (FIRST_X_ASSUM (mp_tac o Q.SPEC `cn`)) >>
+ rw [] >>
+ PairCases_on `tenvC` >>
+ PairCases_on `tenvC'` >>
+ PairCases_on `envC` >>
+ PairCases_on `envC'` >>
+ fs [lookup_con_id_def, merge_tenvC_def, merge_envC_def, merge_def, lookup_append] >>
+ every_case_tac >>
+ fs [lookup_append, id_to_n_def] >>
+ res_tac >>
+ fs [] >>
+ rw []
+
+ metis_tac []
+ *)
 
 val build_tdefs_cons = Q.prove (
 `!tvs tn ctors tds.
   build_tdefs mn ((tvs,tn,ctors)::tds) =
-    (MAP (\(conN,ts). (Short conN, LENGTH ts, TypeId (mk_id mn tn)))
+    (MAP (\(conN,ts). (conN, LENGTH ts, TypeId (mk_id mn tn)))
         ctors) ++ build_tdefs mn tds`,
 rw [build_tdefs_def]);
 
 val build_ctor_tenv_cons = Q.prove (
 `∀tvs tn ctors tds.
   build_ctor_tenv mn ((tvs,tn,ctors)::tds) =
-    (MAP (λ(cn,ts). (Short cn,tvs,ts,TypeId (mk_id mn tn))) ctors ++ build_ctor_tenv mn tds)`,
+    (MAP (λ(cn,ts). (cn,tvs,ts,TypeId (mk_id mn tn))) ctors ++ build_ctor_tenv mn tds)`,
 rw [build_ctor_tenv_def]);
 
 val build_ctor_tenv_empty = Q.store_thm ("build_ctor_tenv_empty",
 `build_ctor_tenv mn [] = []`,
 rw [build_ctor_tenv_def]);
 
+val flat_toCTmap_def = Define `
+flat_toCTmap tenvC = 
+  MAP (\(cn,(tvs,ts,t)). ((cn,t),(tvs,ts))) tenvC`;
+
 val toCTmap_def = Define `
-toCTmap tenvC = MAP (\(cn,(tvs,ts,t)). ((id_to_n cn,t),(tvs,ts))) tenvC`;
+toCTmap tenvC = 
+  FLAT (MAP (\(mn, tenvC). flat_toCTmap tenvC) (FST tenvC)) ++
+  flat_toCTmap (SND tenvC)`;
 
 val tenvC_ok_CTmap = Q.store_thm ("tenvC_ok_CTmap",
 `!tenvC. tenvC_ok tenvC = tenvCT_ok (toCTmap tenvC)`,
- rw [toCTmap_def, EVERY_MEM, tenvC_ok_def, tenvCT_ok_def] >>
- eq_tac >>
- rw [] >>
- fs [MEM_MAP] >>
- rw []
- >- (res_tac >>
-     PairCases_on `y` >>
-     fs [])
- >- (res_tac >> 
-     PairCases_on `e` >>
-     fs []));
+ rw [flat_toCTmap_def, toCTmap_def, EVERY_MEM, tenvC_ok_def, tenvCT_ok_def] >>
+ eq_tac
+ >- (rw [] >>
+     fs [MEM_MAP] >>
+     rw [] >>
+     PairCases_on `tenvC` >>
+     fs [tenvC_ok_def]
+     >- (PairCases_on `e` >>
+         fs [MEM_FLAT, MEM_MAP, EVERY_MEM, flat_tenvC_ok_def] >>
+         rw [] >>
+         PairCases_on `y` >>
+         fs [MEM_MAP] >>
+         rw [] >>
+         PairCases_on `y` >>
+         fs [] >>
+         rw [] >>
+         res_tac >>
+         fs [] >>
+         res_tac >>
+         fs [])
+     >- (PairCases_on `y` >>
+         fs [EVERY_MEM, flat_tenvC_ok_def] >>
+         res_tac >>
+         fs []))
+ >- (PairCases_on `tenvC` >>
+     rw [tenvC_ok_def, flat_tenvC_ok_def, EVERY_MEM]
+     >- (PairCases_on `p` >>
+         rw [] >>
+         PairCases_on `e` >>
+         rw [] >>
+         FIRST_X_ASSUM (mp_tac o Q.SPEC `((e0,e3),e1,e2)`) >>
+         rw [] >>
+         fs [MEM_FLAT, MEM_MAP] >>
+         res_tac >>
+         pop_assum (mp_tac o Q.SPEC `MAP (λ(cn,tvs,ts,t). ((cn,t),tvs,ts)) p1`) >>
+         rw [MEM_MAP] >>
+         res_tac >>
+         fs [MEM_MAP])
+     >- (PairCases_on `e` >>
+         rw [] >>
+         fs [MEM_MAP] >>
+         FIRST_X_ASSUM (mp_tac o Q.SPEC `((e0,e3),e1,e2)`) >>
+         fs [MEM_FLAT, MEM_MAP] >>
+         rw [] >>
+         res_tac >>
+         fs [MEM_MAP])));
 
+         (*
 val check_ctor_tenvC_ok_lem = Q.prove (
 `!mn tenvC c. check_ctor_tenv mn tenvC c ⇒ 
   EVERY (\(cn,tvs,ts,tn). EVERY (check_freevars 0 tvs) ts) (build_ctor_tenv mn c)`,
@@ -1391,7 +1487,7 @@ fs [check_ctor_tenv_def, EVERY_MAP] >|
      fs []] >>
 cases_on `mn` >>
 rw [mk_id_def]);
-
+*)
 (*
 val check_ctor_foldr_flat_map = Q.store_thm ("check_ctor_foldr_flat_map",
 `!c. (FOLDR
@@ -1481,14 +1577,19 @@ val check_dup_ctor_lem2 = Q.prove (
  rw []);
 
 val check_ctor_tenvC_ok = Q.store_thm ("check_ctor_tenvC_ok",
-`!mn tenvC c. check_ctor_tenv mn tenvC c ⇒ tenvC_ok (build_ctor_tenv mn c)`,
- rw [tenvC_ok_def] >>
- imp_res_tac check_ctor_tenvC_ok_lem >>
- fs [EVERY_MEM] >>
+`!mn tenvC c. check_ctor_tenv mn tenvC c ⇒ flat_tenvC_ok (build_ctor_tenv mn c)`,
+ rw [build_ctor_tenv_def, tenvC_ok_def, flat_tenvC_ok_def] >>
+ fs [check_ctor_tenv_def, EVERY_MEM, MEM_FLAT, MEM_MAP] >>
  rw [] >>
- PairCases_on `e` >>
+ PairCases_on `y` >>
+ fs [MEM_MAP] >>
+ rw [] >>
+ PairCases_on `y` >>
+ rw [] >>
+ res_tac >>
  fs [] >>
- rw []);
+ res_tac >>
+ fs []);
 
 val check_dup_ctors_cons = Q.store_thm ("check_dup_ctors_cons",
 `!tvs ts ctors tds.
@@ -1510,8 +1611,9 @@ val check_ctor_tenv_cons = Q.prove (
 `!tvs ts ctors tds tenvC.
   check_ctor_tenv mn tenvC ((tvs,ts,ctors)::tds) ⇒
   check_ctor_tenv mn tenvC tds`,
-rw [check_ctor_tenv_def] >>
-metis_tac [check_dup_ctors_cons]);
+ rw [] >>
+ fs [check_ctor_tenv_def] >>
+ metis_tac [check_dup_ctors_cons]);
 
 val check_ctor_tenv_dups = Q.store_thm ("check_ctor_tenv_dups",
 `!mn tenvC tdecs. check_ctor_tenv mn tenvC tdecs ⇒ check_dup_ctors tdecs`,
@@ -1524,15 +1626,16 @@ val check_ctor_tenv_dups = Q.store_thm ("check_ctor_tenv_dups",
  fs [check_ctor_tenv_def, check_dup_ctors_def, LET_THM]);
 
 val check_ctor_tenvCT_ok = Q.store_thm ("check_ctor_tenvCT_ok",
-`!mn tenvC c. check_ctor_tenv mn tenvC c ⇒ tenvCT_ok (toCTmap (build_ctor_tenv mn c))`,
+`!mn tenvC c. check_ctor_tenv mn tenvC c ⇒ tenvCT_ok (flat_toCTmap (build_ctor_tenv mn c))`,
  rw [] >>
  imp_res_tac check_ctor_tenvC_ok >>
- fs [tenvC_ok_def, tenvCT_ok_def, EVERY_MEM, toCTmap_def, MEM_MAP] >>
+ fs [flat_tenvC_ok_def, tenvCT_ok_def, EVERY_MEM, flat_toCTmap_def, MEM_MAP] >>
  rw [] >>
  res_tac >>
  PairCases_on `y` >>
  fs []);
 
+ (*
 val toCTmap_lookup = Q.prove (
 `!cn tenvC tvs ts t.
   lookup cn tenvC = SOME (tvs,ts,t)
@@ -1545,7 +1648,7 @@ val toCTmap_lookup = Q.prove (
  every_case_tac >>
  rw [] >>
  metis_tac [toCTmap_def]);
-
+ *)
 
 (*
 *
@@ -1568,7 +1671,7 @@ x = (x0,x1)
 *
 * *)
 
-
+(*
 val toCTmap_lookup_lem = Q.prove (
 `!cn mn ctors tvs ts tn t.
   lookup (Short cn) (MAP (λ(cn,ts). (Short cn,tvs,ts,TypeId (mk_id mn tn))) ctors) = NONE
@@ -1653,6 +1756,7 @@ val toCTmap_lookup2 = Q.prove (
      rw [] >>
      imp_res_tac toCTmap_lookup_lem2 >>
      fs [id_to_n_def, toCTmap_def]));
+     *)
 
 val ctor_env_to_tdefs = Q.prove (
 `!mn tds cn n t tvs ts.
@@ -1674,17 +1778,26 @@ val ctor_env_to_tdefs = Q.prove (
  every_case_tac >>
  rw []);
 
+ (*
 val toCTmap_append = Q.store_thm ("toCTmap_append",
-`!x y. toCTmap (x++y) = toCTmap x ++ toCTmap y`,
-rw [toCTmap_def]);
+`!x y. toCTmap (merge_tenvC x y) = toCTmap x ++ toCTmap y`,
 
+ rw [toCTmap_def] >>
+ PairCases_on `x` >>
+ PairCases_on `y` >>
+ rw [merge_tenvC_def, flat_toCTmap_def, merge_def, MAP_FLAT]
+
+);
+*)
+
+(*
 val check_ctor_disjoint_env = Q.store_thm ("check_ctor_disjoint_env",
 `!mn tenvC tds.
   check_ctor_tenv mn tenvC tds
   ⇒
-  disjoint_env (toCTmap (build_ctor_tenv mn tds)) (toCTmap tenvC)`,
+  disjoint_env (flat_toCTmap (build_ctor_tenv mn tds)) (toCTmap tenvC)`,
  induct_on `tds` >>
- rw [build_ctor_tenv_empty, toCTmap_def]
+ rw [build_ctor_tenv_empty, flat_toCTmap_def]
  >- rw [disjoint_env_def, DISJOINT_DEF] >>
  `?tvs tn ctors. h = (tvs,tn,ctors)` by (PairCases_on `h` >> rw []) >>
  rw [build_ctor_tenv_cons] >>
@@ -1693,7 +1806,7 @@ val check_ctor_disjoint_env = Q.store_thm ("check_ctor_disjoint_env",
  fs [disjoint_env_def, DISJOINT_DEF, EXTENSION] >>
  rw [] >>
  pop_assum (ASSUME_TAC o Q.SPEC `x`) >>
- fs [toCTmap_def] >>
+ fs [flat_toCTmap_def] >>
  fs [MAP_MAP_o, combinTheory.o_DEF, MEM_MAP] >>
  CCONTR_TAC >>
  fs [] >>
@@ -1705,10 +1818,14 @@ val check_ctor_disjoint_env = Q.store_thm ("check_ctor_disjoint_env",
  rw [] >>
  fs [] >>
  rw [] >>
+ PairCases_on `tenvC` >>
  fs [check_ctor_tenv_def, EVERY_MEM] >>
  res_tac >>
- fs []);
+ fs [toCTmap_def] >>
+ rw []);
+ *)
 
+ (*
 val extend_consistent_con = Q.store_thm ("extend_consistent_con",
 `!envC tenvC tds.
   check_ctor_tenv mn tenvC tds ∧
@@ -1742,6 +1859,7 @@ val extend_consistent_con = Q.store_thm ("extend_consistent_con",
      >- metis_tac [ctor_env_to_tdefs, SOME_11, PAIR_EQ,toCTmap_lookup] 
      >- metis_tac [toCTmap_lookup2, ctor_env_to_tdefs, SOME_11, PAIR_EQ,toCTmap_lookup] 
      >- metis_tac [ctor_env_to_tdefs, SOME_11, PAIR_EQ]));
+     *)
 
 val lemma = Q.prove (
 `!f a b c. (\(x,y,z). f x y z) (a,b,c) = f a b c`,
@@ -1894,6 +2012,7 @@ rw [] >|
      fs [bvl2_append, merge_def, num_tvs_bvl2] >>
      metis_tac [tenv_ok_bvl2]]);
 
+     (*
 val type_d_tenvCT_ok = Q.store_thm ("type_d_tenvCT_ok",
 `!tvs tenvM tenvC tenv d tenvC' tenv' tenvM'' tenvC''.
   type_d tvs tenvM tenvC tenv d tenvC' tenv'
@@ -1945,6 +2064,7 @@ val type_ds_tenvCT_ok = Q.store_thm ("type_ds_tenvCT_ok",
      fs [num_tvs_bvl2, merge_def, disjoint_env_def, DISJOINT_DEF, EXTENSION] >>
      rw [] >>
      metis_tac []));
+     *)
 
 val type_specs_tenv_ok = Q.store_thm ("type_specs_tenv_ok",
 `!tvs tenvC tenv specs tenvC' tenv'.
